rustfrontend/ElaborateDropProof.v
@@ -8,11 +8,11 @@ Require Import Rusttypes.
 Require Import Errors.
 Require Import LanguageInterface CKLR Inject InjectFootprint.
 Require Import InitDomain InitAnalysis ElaborateDrop.
-Require Import Rustlight RustIR RustOp.
+Require Import Rustlight Rustlightown RustIR RustOp.
 Require Import RustIRsem RustIRown RustIRcfg.
 
 Import ListNotations.
-
+Local Open Scope list_scope.
 Local Open Scope error_monad_scope.
 
 Record match_prog (p tp: RustIR.program) : Prop := {
@@ -60,7 +60,95 @@ Admitted.
 End INJECT.
 End MATCH_PROGRAMS.
 
-    
+
+Inductive match_drop_place_state : option drop_place_state -> statement -> Prop :=
+| match_dps_none:
+  match_drop_place_state None Sskip
+| match_dps_comp: forall p l,
+    (* step_dropplace_init2 has simulated the drop flag condition
+    checking *)
+    match_drop_place_state (Some (drop_fully_owned_comp p l)) (Ssequence (Sdrop p) (makeseq (map (fun p => Sdrop p) l)))
+| match_dps_box: forall l,
+    match_drop_place_state (Some (drop_fully_owned_box l)) (makeseq (map (fun p => Sdrop p) l))
+.
+
+(* Because in dropplace state we do not know the pc, so we use own_env
+to establish the relation between split drop places and target
+statement. This relation should be proved when we enter Dropplace
+state *)
+Inductive match_split_drop_places flagm : own_env -> list (place * bool) -> statement -> Prop :=
+| match_sdp_nil: forall own,
+    match_split_drop_places flagm own nil Sskip
+| match_sdp_cons_flag: forall p flag own l ts full
+    (FLAG: get_dropflag_temp flagm p = Some flag)
+    (SPLIT: match_split_drop_places flagm (move_place own p) l ts),
+    (* how to ensure that p is owned in own_env *)    
+    match_split_drop_places flagm own ((p,full)::l) (Ssequence (generate_drop p full (Some flag)) ts)
+| match_sdp_cons_must_init: forall p own l ts full
+    (FLAG: get_dropflag_temp flagm p = None)
+    (SPLIT: match_split_drop_places flagm (move_place own p) l ts)
+    (OWN: is_owned own p = true),
+    (* how to ensure that p is owned in own_env *)    
+    match_split_drop_places flagm own ((p,full)::l) (Ssequence (generate_drop p full None) ts)
+| match_sdp_cons_must_uninit: forall p own l ts full
+    (FLAG: get_dropflag_temp flagm p = None)
+    (SPLIT: match_split_drop_places flagm (move_place own p) l ts)
+    (OWN: is_owned own p = false),
+    (* how to ensure that p is owned in own_env *)    
+    match_split_drop_places flagm own ((p,full)::l) (Ssequence Sskip ts)
+.
+
+
+Section MATCH_CONT.
+  
+Context {AN: Type} {An: Type} (get_an: AN -> node -> An).
+Context (ae: AN).
+Context (transl_stmt: An -> statement -> Errors.res statement).
+
+Let match_stmt := match_stmt get_an ae transl_stmt.
+
+Variable j: meminj.
+
+Inductive match_cont  : statement -> rustcfg -> cont -> RustIRsem.cont -> node -> option node -> option node -> node -> Prop :=
+| match_Kseq: forall body cfg s ts k tk pc next cont brk nret
+    (MSTMT: match_stmt body cfg s ts pc next cont brk nret)
+    (MCONT: match_cont body cfg k tk next cont brk nret),
+    match_cont body cfg (Kseq s k) (RustIRsem.Kseq ts tk) pc cont brk nret
+| match_Kstop: forall body cfg nret
+    (RET: cfg ! nret = Some Iend),
+    match_cont body cfg Kstop RustIRsem.Kstop nret None None nret
+| match_Kloop: forall body cfg s ts k tk body_start loop_jump_node exit_loop nret contn brk
+    (START: cfg ! loop_jump_node = Some (Inop body_start))
+    (MSTMT: match_stmt body cfg s ts body_start loop_jump_node (Some loop_jump_node) (Some exit_loop) nret)
+    (MCONT: match_cont body cfg k tk exit_loop contn brk nret),
+    match_cont body cfg (Kloop s k) (RustIRsem.Kloop ts tk) loop_jump_node (Some loop_jump_node) (Some exit_loop) nret
+| match_Kcall: forall body cfg k tk nret f tf le tle own p
+    (MSTK: match_stacks (Kcall p f le own k) (RustIRsem.Kcall p tf tle tk))
+    (RET: cfg ! nret = Some Iend),
+    (* in the end of a function *)
+    match_cont body cfg (Kcall p f le own k) (RustIRsem.Kcall p tf tle tk) nret None None nret
+| match_Kdropcall: forall body cfg k tk pc cont brk nret st membs b tb ofs tofs id
+    (INJ: Val.inject j (Vptr b ofs) (Vptr tb tofs))
+    (MCONT: match_cont body cfg k tk pc cont brk nret),
+    match_cont body cfg (Kdropcall id (Vptr b ofs) st membs k) (RustIRsem.Kdropcall id (Vptr tb tofs) st membs tk) pc cont brk nret
+| match_Kdorpplace: forall body f tf st l k tk e te own flagm cfg nret cont brk pc ts1 ts2
+    (MCONT: match_cont f.(fn_body) cfg k tk pc cont brk nret)    
+    (MDPS: match_drop_place_state st ts1)
+    (MSPLIT: match_split_drop_places flagm own l ts2),
+    (* source program: from dropplace to droopstate, target: from
+    state to dropstate. So Kdropplace matches Kcall *)
+    match_cont body cfg (Kdropplace f st l e own k) (RustIRsem.Kcall None tf te (RustIRsem.Kseq (Ssequence ts1 ts2) tk)) pc cont brk nret 
+               
+with match_stacks : cont -> RustIRsem.cont -> Prop :=
+| match_stacks_stop: match_stacks Kstop (RustIRsem.Kstop)
+| match_stacks_call: forall f tf nret cfg pc contn brk k tk own p le tle
+    (TRFUN: tr_fun f nret cfg)
+    (MCONT: match_cont f.(fn_body) cfg k tk pc contn brk nret),
+    match_stacks (Kcall p f le own k) (RustIRsem.Kcall p tf tle tk)
+.
+
+End MATCH_CONT.
+
 Section PRESERVATION.
 
 Variable prog: program.
@@ -74,14 +162,24 @@ Let ge := globalenv se prog.
 Let tge := globalenv tse tprog.
 Let ce := ge.(genv_cenv).
 
+
 Inductive match_states: state -> RustIRsem.state -> Prop := 
-  | match_regular_state:
-    forall f s k e own m tf ts tk te tm j flagm
-      (AN: analyze ce f = OK (maybeInit, maybeUninit, universe))
-      (MSTMT: el_stmt ce maybeInit maybeUninit universe flagm f.(fn_body) cfg s ts)
-      (MCONT: el_cont 
-      (MINJ: Mem.inject j m tm),
-      match_states (State f s k e own m) (RustIRsem.State tf ts tk te tm). 
+| match_regular_state:
+  forall f s k e own m tf ts tk te tm j flagm maybeInit maybeUninit universe cfg nret cont brk next pc
+    (AN: analyze ce f = OK (maybeInit, maybeUninit, universe))
+    (TRFUN: tr_fun f nret cfg)
+    (MSTMT: match_stmt get_init_info (maybeInit, maybeUninit, universe) (elaborate_stmt flagm ce) f.(fn_body) cfg s ts pc next cont brk nret)
+    (MCONT: match_cont get_init_info (maybeInit, maybeUninit, universe) (elaborate_stmt flagm ce) j f.(fn_body) cfg k tk next cont brk nret)
+    (MINJ: Mem.inject j m tm),
+    match_states (State f s k e own m) (RustIRsem.State tf ts tk te tm)
+| match_drppplace: forall f tf st l k tk e te own m tm j flagm  maybeInit maybeUninit universe cfg nret cont brk next ts1 ts2
+    (MCONT: match_cont get_init_info (maybeInit, maybeUninit, universe) (elaborate_stmt flagm ce) j f.(fn_body) cfg k tk next cont brk nret)    
+    (MDPS: match_drop_place_state st ts1)
+    (MSPLIT: match_split_drop_places flagm own l ts2)
+    (MINJ: Mem.inject j m tm),
+    match_states (Dropplace f st l k e own m) (RustIRsem.State tf ts1 (RustIRsem.Kseq ts2 tk) te tm)
+
+. 
 
 
 Lemma step_simulation:
